code/sha3/Hacl.Spec.SHA3.Vec.Common.fst
@@ -9,27 +9,19 @@ open Lib.LoopCombinators
 
 open Spec.SHA3.Constants
 
-#reset-options "--z3rlimit 50 --max_fuel 0 --max_ifuel 0"
-
 noextract
 type m_spec =
   | M32
-  | M128
   | M256
 
 inline_for_extraction noextract
-let lanes_t = n:nat{n == 1 \/ n == 2 \/ n == 4}
+let lanes_t = n:nat{n == 1 \/ n == 4}
 
 inline_for_extraction noextract
 let lanes (m:m_spec) : lanes_t =
   match m with
-  | M128 -> 2
+  | M32 -> 1
   | M256 -> 4
-  | _ -> 1
-
-noextract
-let is_supported (m:m_spec) =
-  lanes m = 1 \/ lanes m = 4
 
 inline_for_extraction noextract
 let element_t (m:m_spec) = vec_t U64 (lanes m)
@@ -43,10 +35,10 @@ val load_element: m:m_spec -> uint_t U64 SEC -> element_t m
 let load_element m x = vec_load x (lanes m)
 
 inline_for_extraction noextract
-let next_block_seq_zero (m:m_spec{is_supported m}) :
+let next_block_seq_zero (m:m_spec) :
   Lib.MultiBuffer.multiseq (lanes m) 256 =
-  match lanes m with
-  | 1 -> Lib.NTuple.ntup1 (create 256 (u8 0))
-  | 4 ->
+  match m with
+  | M32 -> Lib.NTuple.ntup1 (create 256 (u8 0))
+  | M256 ->
     let b = create 256 (u8 0) in
     Lib.NTuple.ntup4 (b, (b, (b, b)))
